Syntax.thy
@@ -1,5 +1,5 @@
 theory Syntax
-  imports Main
+  imports Main State
 begin
 
 chapter \<open>While Language Syntax\<close>
@@ -33,7 +33,7 @@ datatype ('a,'b) com =
   | Loop "('a,'b) com" ("_*" [100] 150)
   | Parallel "('a,'b) com" "('a,'b) com"  (infixr "||" 150)
   | Thread "('a,'b) com"
-  (* | Capture 'b "('a,'b) com" *)
+  | Capture 'b "('a,'b) com"
   (* | CaptureAll "('a,'b) com" *)
 
 
@@ -46,32 +46,156 @@ fun local :: "('a,'b) com \<Rightarrow> bool"
     "local (c\<^sub>1 \<cdot> c\<^sub>2) = (local c\<^sub>1 \<and> local c\<^sub>2)" |
     "local (c\<^sub>1 \<sqinter> c\<^sub>2) = (local c\<^sub>1 \<and> local c\<^sub>2)" |  
     "local (c*) = (local c)" |    
-    (* "local (Capture _ c) = local c" | *)
+    "local (Capture k c) = local c" |
     (* "local (CaptureAll c) = local c" | *)
     "local _ = True"
 
 
 class state =
-  fixes merge :: "'a \<Rightarrow> 'a \<Rightarrow> 'a"
-  (* assumes "surj (\<lambda>m. merge m s)" *)
+  (* takes key, initial outer state, then returns inner state *)
+  fixes push :: "'a \<Rightarrow> 'a \<Rightarrow> 'a"
+  (* takes key, initial outer state, final outer state, and returns final inner state. *)
+  fixes popl :: "'a \<Rightarrow> 'a"
+  fixes popr :: "'a \<Rightarrow> 'a"
+  assumes popl_push [simp]: "popl (push a b) = a"
+  assumes popr_push [simp]: "popr (push a b) = b"
+  assumes push_intro: "\<exists>m. m' = push m s"
 
-fun capBasic :: "('a,'b :: state) basic \<Rightarrow> 'b \<Rightarrow> 'b \<Rightarrow> ('a,'b) basic" where
-"capBasic \<alpha> s s' = 
-  (tag \<alpha>, {m. merge m s \<in> vc \<alpha>}, {(m,m'). (merge m s, merge m' s') \<in> beh \<alpha>})"
-
-fun uncapBasic :: "'b \<Rightarrow> ('a,'b :: state) basic \<Rightarrow> ('a,'b) basic" where
-"uncapBasic s \<alpha> = 
-  (tag \<alpha>, {merge m s |m. m \<in> vc \<alpha>}, {(merge m s, merge m' s) |m m'. (m,m') \<in> beh \<alpha>})"
-
-lemma "surj f \<Longrightarrow> {f a |a. f a \<in> A} = A"
+lemma push_intro_fun: 
+  "\<exists>f. m' = push (f m' s) s"
+using push_intro
 by fast
 
-lemma "(uncapBasic s (capBasic \<alpha> s s)) = \<alpha>"
-apply auto
-oops
+
+fun uncapPred :: "('b::state) \<Rightarrow> 'b set \<Rightarrow> 'b set" where
+"uncapPred s P = {push m s |m. m \<in> P}"
+
+fun capPred :: "('b::state) set \<Rightarrow> 'b set" where
+"capPred P = {popl m |m. m \<in> P}"
+
+
+fun capBeh :: "('b::state) \<Rightarrow> 'b rel \<Rightarrow> 'b rel" where
+"capBeh s b = {(popl m,popl m') |m m'. (m,m') \<in> b}" 
+
+fun uncapBeh :: "('b::state) \<Rightarrow> 'b rel \<Rightarrow> 'b rel" where
+"uncapBeh s b = {(push m s,push m' s) |m m'. (m,m') \<in> b}" 
+
+
+(* captures and hides the local effects of a basic. 
+goes from local to global.  *)
+fun capBasic :: "('b::state) \<Rightarrow> ('a,'b) basic \<Rightarrow> ('a,'b) basic" where
+"capBasic s \<alpha> = (tag \<alpha>, capPred (vc \<alpha>), capBeh s (beh \<alpha>))"
+
+(* uncaptures and makes visible the effects of a basic. 
+goes from global to local context. *)
+fun uncapBasic :: "('b::state) \<Rightarrow> ('a,'b) basic \<Rightarrow> ('a,'b) basic" where
+"uncapBasic s \<alpha> = (tag \<alpha>, uncapPred s (vc \<alpha>), uncapBeh s (beh \<alpha>))"
+
+fun capRely :: "('b::state) rel \<Rightarrow> 'b rel" where
+"capRely R = {(popl m, popl m') |m m'. (m,m') \<in> R}"
+
+fun uncapRely :: "('b::state) rel \<Rightarrow> 'b rel" where
+"uncapRely R = {(push m s, push m' s) |m m' s. (m,m') \<in> R}"
+
+
+fun uncapGuar :: "('b::state) rel \<Rightarrow> 'b rel" where
+"uncapGuar G = {(push m s, push m' s') |m m' s s'. (m,m') \<in> G}"
+
+fun capGuar :: "('b::state) rel \<Rightarrow> 'b rel" where
+"capGuar G = {(popl m, popl m') |m m'. (m,m') \<in> G}"
+
+lemma cap_uncapBeh: "capBeh s (uncapBeh s b) = b"
+by (auto, metis popl_push)
+
+lemma cap_uncapPred: "capPred (uncapPred s P) = P"
+by (auto, metis popl_push)
+
+lemma cap_uncapBasic: "capBasic s (uncapBasic s \<alpha>) = \<alpha>"
+using cap_uncapPred[of s "vc \<alpha>"]
+using cap_uncapBeh[of s "beh \<alpha>"]
+by simp
+
+lemma uncap_capGuar: "uncapGuar (capGuar G) = G"
+by auto (metis (full_types) popr_push push_intro)+
+
+lemma capPred_mono: "P \<subseteq> P' \<Longrightarrow> capPred P \<subseteq> capPred P'"
+by auto
+
+lemma uncapGuar_mono: "G \<subseteq> G' \<Longrightarrow> uncapGuar G \<subseteq> uncapGuar G'"
+by auto
+
+lemma uncapGuar_inter: "uncapGuar (G \<inter> G') = uncapGuar G \<inter> uncapGuar G'"
+by auto (metis (full_types) popr_push push_intro)+
+
+lemma stable_uncap: "stable (uncapRely R) (uncapPred s P) \<Longrightarrow> stable R P"
+unfolding stable_def
+by (auto, metis popl_push)
+
+lemma image_of_some:
+  assumes "\<forall>m. \<exists>x. m = f x"
+  shows "P = f ` {SOME x. m = f x |m. m \<in> P}"
+proof
+  show "P \<subseteq> f ` {SOME x. m = f x |m. m \<in> P}"
+  using assms someI_ex by fast
+next
+  show "P \<supseteq> f ` {SOME x. m = f x |m. m \<in> P}"
+  using assms someI_ex
+  by (smt (verit, ccfv_SIG) image_Collect_subsetI)
+qed
+
+lemma uncap_exists: "\<exists>P'. P = uncapPred s P'"
+proof
+  show "P = uncapPred s {SOME x. m = push x s |m. m \<in> P}"
+    using image_of_some[of "\<lambda>x. push x s" P] push_intro by auto
+qed
+
+(* captures the effect of a command *)
+fun capCom :: "('b::state) \<Rightarrow> ('a,'b) com \<Rightarrow> ('a,'b) com" where
+    "capCom k (Basic \<beta>) = Basic (capBasic k \<beta>)" |
+    "capCom k (Seq c\<^sub>1 c\<^sub>2) = Seq (capCom k c\<^sub>1) (capCom k c\<^sub>2)" |
+    "capCom k (Ord c\<^sub>1 c\<^sub>2) = Ord  (capCom k c\<^sub>1) (capCom k c\<^sub>2)" |
+    "capCom k (Choice c\<^sub>1 c\<^sub>2) = Choice  (capCom k c\<^sub>1) (capCom k c\<^sub>2)" |
+    "capCom k (SeqChoice S) = SeqChoice (map (uncapBasic k) ` S)" |
+    "capCom k (Parallel c\<^sub>1 c\<^sub>2) = Parallel (capCom k c\<^sub>1) (capCom k c\<^sub>2)" |
+    "capCom k (Loop c) = Loop (capCom k c)" |
+    "capCom k (Thread c) = Thread (capCom k c)" |
+    (* "capCom k (Capture s c) = uncapBasic s ` capCom k c" | *)
+    "capCom k (Capture k' c) = Capture k (capCom k' c)" |
+    "capCom _ Nil = Nil"
+
+fun uncapCom :: "('b::state) \<Rightarrow> ('a,'b) com \<Rightarrow> ('a,'b) com" where
+    "uncapCom k (Basic \<beta>) = Basic (uncapBasic k \<beta>)" |
+    "uncapCom k (Seq c\<^sub>1 c\<^sub>2) = Seq (uncapCom k c\<^sub>1) (uncapCom k c\<^sub>2)" |
+    "uncapCom k (Ord c\<^sub>1 c\<^sub>2) = Ord  (uncapCom k c\<^sub>1) (uncapCom k c\<^sub>2)" |
+    "uncapCom k (Choice c\<^sub>1 c\<^sub>2) = Choice  (uncapCom k c\<^sub>1) (uncapCom k c\<^sub>2)" |
+    "uncapCom k (SeqChoice S) = SeqChoice (map (uncapBasic k) ` S)" |
+    "uncapCom k (Parallel c\<^sub>1 c\<^sub>2) = Parallel (uncapCom k c\<^sub>1) (uncapCom k c\<^sub>2)" |
+    "uncapCom k (Loop c) = Loop (uncapCom k c)" |
+    "uncapCom k (Thread c) = Thread (uncapCom k c)" |
+    (* "capCom k (Capture s c) = uncapBasic s ` capCom k c" | *)
+    "uncapCom k (Capture k' c) = Capture k' (uncapCom k' c)" |
+    "uncapCom _ Nil = Nil"
+    (* "basics (CaptureAll c) = basics c" | *)
+
+
+definition thr\<^sub>\<alpha> :: "'b merge \<Rightarrow> 'b \<Rightarrow> 'b \<Rightarrow> ('a,'b) basic \<Rightarrow> ('a,'b) basic" where
+"thr\<^sub>\<alpha> op l l' \<alpha> \<equiv> (tag \<alpha>, thr\<^sub>P op l (vc \<alpha>), thr2glb op l l' (beh \<alpha>))"
+
+(* fun thr\<^sub>c :: "'b merge \<Rightarrow> 'b \<Rightarrow> 'b \<Rightarrow> ('a,'b) com \<Rightarrow> ('a,'b) com" where
+"thr\<^sub>c op l l' (Basic \<beta>) = Basic (thr\<^sub>\<alpha> op l l' \<beta>)" |
+"thr\<^sub>c op l l' (Seq c\<^sub>1 c\<^sub>2) = Seq (thr\<^sub>c op l l' c\<^sub>1) (thr\<^sub>c op l l' c\<^sub>2)" |
+"thr\<^sub>c op l l' (Ord c\<^sub>1 c\<^sub>2) = Ord (thr\<^sub>c op l l' c\<^sub>1) (thr\<^sub>c op l l' c\<^sub>2)" |
+"thr\<^sub>c op l l' (Choice c\<^sub>1 c\<^sub>2) = Choice (thr\<^sub>c op l l' c\<^sub>1) (thr\<^sub>c op l l' c\<^sub>2)" |
+"thr\<^sub>c op l l' (SeqChoice S) = SeqChoice (map (thr\<^sub>\<alpha> op l l') ` S)" |
+"thr\<^sub>c op l l' (Parallel c\<^sub>1 c\<^sub>2) = Parallel (thr\<^sub>c op l l' c\<^sub>1) (thr\<^sub>c op l l' c\<^sub>2)" |
+"thr\<^sub>c op l l' (Loop c) = Loop (thr\<^sub>c op l l' c)" |
+"thr\<^sub>c op l l' (Thread c) = Thread (thr\<^sub>c op l l' c)" |
+"thr\<^sub>c op l l' (Capture op2 k k' c) = Capture op l l' (thr\<^sub>c op2 k k' c)" |
+"thr\<^sub>c op l l' Nil = Nil" *)
+(* "basics (CaptureAll c) = basics c" | *)
 
 text \<open>Identify all operations in a program\<close>
-fun basics :: "('a,'b ) com \<Rightarrow> ('a,'b) basic set"
+fun basics :: "('a,'b::state) com \<Rightarrow> ('a,'b) basic set"
   where
     "basics (Basic \<beta>) = {\<beta>}" |
     "basics (Seq c\<^sub>1 c\<^sub>2) = basics c\<^sub>1 \<union> basics c\<^sub>2" |
@@ -82,9 +206,12 @@ fun basics :: "('a,'b ) com \<Rightarrow> ('a,'b) basic set"
     "basics (Loop c) = basics c" |
     "basics (Thread c) = basics c" |
     (* "basics (Capture s c) = uncapBasic s ` basics c" | *)
-    (* "basics (Capture s c) = basics c" |  *)
+    "basics (Capture k c) = capBasic k ` basics c" |
     (* "basics (CaptureAll c) = basics c" | *)
     "basics _ = {}"
+
+(* lemma basics_thr\<^sub>c: "basics (thr\<^sub>c op l l' c) = thr\<^sub>\<alpha> op l l' ` basics c"
+by (induct c arbitrary: op l l') auto *)
 
 text \<open>Shorthand for an environment step\<close>
 abbreviation Env :: "'b rel \<Rightarrow> ('a,'b) com"
